examples/invariants/DY.Example.Invariants.Uniqueness.Init.fst
@@ -1,0 +1,127 @@
+module DY.Example.Invariants.Uniqueness.Init
+
+open Comparse
+open DY.Core
+module L = DY.Lib
+// module List = FStar.List.Tot.Base
+// module Trace = DY.Core.Trace.Type
+open DY.Example.Invariants.Uniqueness
+
+
+let prop_state_on (#a:Type) (#state_t:Type) {|ps_state : parseable_serializeable bytes state_t|} 
+  (from_state: state_t  -> a) (p: a -> bool ) (state:state_raw) : prop =
+  match parse state_t state with
+  | None -> True
+  | Some state -> p (from_state state)
+
+let prop_on_idn (f: nat -> bool) (state:state_raw) : prop =
+  prop_state_on
+      (fun state -> state.idn)
+      f
+      state
+
+let forall_idns (f: nat -> bool) (sess:session_raw) : prop =
+  forall_rev_list (prop_on_idn f) sess
+  
+
+let idn_does_not_appear_in_session (idn:nat) (sess:session_raw) : prop =
+  forall_idns (fun idn' -> idn <> idn') sess
+
+val max_id_in_session_largest:
+  sess:session_raw ->
+  Lemma 
+  ( let m_idn = find_max_id_in_session sess in
+    forall_idns (fun idn -> m_idn >= idn) sess
+  )
+let rec max_id_in_session_largest sess = 
+  let m_idn = find_max_id_in_session sess in
+  match sess with
+  | Nil -> ()
+  | Snoc rest state ->
+      max_id_in_session_largest rest
+
+let forall_sessions (p:session_raw ->  prop) (fst:full_state_raw) : prop =
+  forall sid sess. (sid, sess) `List.mem` fst ==> p sess
+
+let idn_does_not_appear_in_full_state (idn:nat) (fst:full_state_raw) : prop =
+  forall_sessions (idn_does_not_appear_in_session idn) fst
+
+
+val curr_max_id_largest :
+  fst:full_state_raw ->
+  Lemma 
+  ( let c_max = find_curr_max_id fst in
+    forall_sessions (forall_idns (fun idn -> c_max >= idn)) fst    
+  )
+let rec curr_max_id_largest fst =
+  let c_max = find_curr_max_id fst in
+  match fst with
+  | [] -> ()
+  | (_, sess) :: rest ->
+        max_id_in_session_largest sess;
+        curr_max_id_largest rest
+
+val new_idn_does_not_appear_in_full_state: p:principal -> tr:trace ->
+  Lemma
+  (requires has_full_state_for tr p
+  )
+  (ensures (
+    let (n_idn,_) = new_idn p tr in
+    let fst = access_full_state tr p in
+    n_idn `idn_does_not_appear_in_full_state` fst
+  ))
+let new_idn_does_not_appear_in_full_state p tr =
+  let fst = access_full_state tr p in
+  curr_max_id_largest fst
+
+
+#push-options "--z3rlimit 20"
+val init_invariant: tr:trace -> p:principal ->
+  Lemma 
+    (requires trace_invariant tr)
+    (ensures  (
+      let (_,tr_out) = init p tr in
+      trace_invariant tr_out
+      )
+    )
+let init_invariant tr p =
+  let (idn, tr_after_new_idn) = new_idn p tr in
+  let new_state = S idn 0 in
+  let new_state_b = serialize p_state new_state in
+  let (new_sess_id, tr_after_new_session) = set_new_session p (serialize p_state new_state) tr_after_new_idn in
+  serialize_wf_lemma p_state (is_knowable_by (principal_state_label p new_sess_id) tr_after_new_idn) new_state;
+
+  match fst (get_full_state p tr) with
+  | None -> ()
+  | Some full_st ->
+  introduce forall sess. sess `List.mem` full_st ==> (
+    match sess with
+    | (_, Nil) -> True
+    | (sid_i, Snoc init_i last_i) -> begin
+              match parse p_state last_i with
+                    | None -> True
+                    | Some last_i ->
+                        if sid_i = new_sess_id
+                          then last_i.idn = idn
+                          else last_i.idn <> idn
+                 end
+    )
+    with (
+      introduce _ ==> _
+      with _ . (
+        match sess with
+        | (_, Nil) -> ()
+        | (sid_i, Snoc init_ last_i) -> 
+             match parse p_state last_i with
+             | None -> ()
+             | Some last_i -> 
+                 set_new_session_new_sid p new_state_b tr;
+                 full_state_mem_get_session_get_state_forall p tr;
+                 assert(sid_i <> new_sess_id);
+                 new_idn_does_not_appear_in_full_state p tr
+
+      )
+    )
+
+
+    
